Makefile
@@ -1,0 +1,31 @@
+# KNOWNTARGETS will not be passed along to CoqMakefile
+KNOWNTARGETS := CoqMakefile doc src/html
+# KNOWNFILES will not get implicit targets from the final rule, and so
+# depending on them won't invoke the submake
+# Warning: These files get declared as PHONY, so any targets depending
+# on them always get rebuilt
+KNOWNFILES   := Makefile src/_CoqProject
+
+.DEFAULT_GOAL := invoke-coqmakefile
+
+CoqMakefile: Makefile src/_CoqProject
+	cd src/; $(COQBIN)coq_makefile -f _CoqProject -o CoqMakefile 
+
+invoke-coqmakefile: CoqMakefile
+	cd src/; $(MAKE) -f CoqMakefile $(filter-out $(KNOWNTARGETS),$(MAKECMDGOALS))
+
+doc: CoqMakeFile
+	cd src/; $(MAKE) -f CoqMakefile $(filter-out $(KNOWNTARGETS),$(MAKECMDGOALS)) gallinahtml
+	rm -rf doc
+	mv src/html ./doc
+
+
+.PHONY: invoke-coqmakefile $(KNOWNFILES)
+
+####################################################################
+##                      Your targets here                         ##
+####################################################################
+
+# This should be the last rule, to handle any targets not declared above
+%: invoke-coqmakefile
+	@true
